galois/network/network_implementation.lean
@@ -134,6 +134,43 @@ def initial_incoming_items : incoming_items
   := { sockets := []
      , messages := [] }
 
+def next_agent_receive_from_label (a_ip : ip) (a : agent)
+  (ports : list port) (sockets : list socket) (bound : time)
+  (incoming : incoming_items)
+  (cont : poll_result ports sockets bound → act a.state_type)
+  (elapsed_fin : fin bound) (rn : remote_name)
+  : poll_receive_label → option (act a.state_type × (global_state_t → global_state_t))
+| poll_receive_label.drop_connection := none
+| poll_receive_label.new_connection :=
+  match list.member_st_decide 
+    (λ s : socket_info, s.server = a_ip ∧ s.new) incoming.sockets with
+  | (sum.inl m) := 
+    let m' := m.to_member in
+    let s := m'.value in
+    match list.check_member s.port ports with
+    | (some portidx) := some (cont (poll_result.new_connection elapsed_fin portidx s.socket)
+      , lookup_updatef a_ip (λ inc, {inc with sockets := list.update_member ({s with new := false}) _ m'})
+      )
+    | none := none
+    end
+  
+  | (sum.inr contra) := none
+  end
+| (poll_receive_label.receive_message mess) :=
+-- OOPS, need to fix: to receive message, I should already have been
+-- informed of the new connection that the message has transferred over
+  match list.member_st_decide (λ p : socket × message_t, p.snd = mess) incoming.messages with
+  | (sum.inl idx) := let idx' := idx.to_member in
+    let p := idx'.value in
+        match list.check_member p.fst sockets with --any other checks necessary?
+        | (some sockidx) := some
+        (cont (poll_result.message elapsed_fin sockidx mess)
+        , lookup_updatef a_ip (λ inc, {inc with messages := list.remove_member _ idx'}))
+        | none := none
+        end
+  | (sum.inr contra) := none
+  end
+
 def next_agent_poll_state_from_label (a_ip : ip) (a : agent)
   (ports : list port) (sockets : list socket) (bound : time)
   (incoming : incoming_items)
@@ -143,38 +180,8 @@ def next_agent_poll_state_from_label (a_ip : ip) (a : agent)
 | (poll_label.receive elapsed rn receive_label) := 
   if H : elapsed < bound 
     then let elapsed_fin : fin bound := ⟨ elapsed, H ⟩ in
-     match receive_label with
-     | poll_receive_label.drop_connection := none
-     | poll_receive_label.new_connection :=
-       match list.member_st_decide 
-         (λ s : socket_info, s.server = a_ip ∧ s.new) incoming.sockets with
-      | (sum.inl m) := 
-         let m' := m.to_member in
-         let s := m'.value in
-         match list.check_member s.port ports with
-         | (some portidx) := some (cont (poll_result.new_connection elapsed_fin portidx s.socket)
-            , lookup_updatef a_ip (λ inc, {inc with sockets := list.update_member ({s with new := false}) _ m'})
-            )
-         | none := none
-         end
-        
-      | (sum.inr contra) := none
-      end
-     | (poll_receive_label.receive_message mess) :=
-      -- OOPS, need to fix: to receive message, I should already have been
-      -- informed of the new connection that the message has transferred over
-        match list.member_st_decide (λ p : socket × message_t, p.snd = mess) incoming.messages with
-        | (sum.inl idx) := let idx' := idx.to_member in
-          let p := idx'.value in
-              match list.check_member p.fst sockets with --any other checks necessary?
-              | (some sockidx) := some
-              (cont (poll_result.message elapsed_fin sockidx mess)
-              , lookup_updatef a_ip (λ inc, {inc with messages := list.remove_member _ idx'}))
-              | none := none
-              end
-        | (sum.inr contra) := none
-        end
-     end
+      next_agent_receive_from_label a_ip a ports
+        sockets bound incoming cont elapsed_fin rn receive_label
    else none
 
 def add_socket (s : socket_info) (a_ip : ip) : global_state_t → global_state_t :=
@@ -183,10 +190,10 @@ def add_message (rn : remote_name) (m : message_t) (a_ip : ip)
   : global_state_t → global_state_t :=
   lookup_updatef a_ip (λ i : incoming_items, {i with messages := (rn, m) :: i.messages })
 
+section
+parameters (a_ip : ip) (a : agent) (incoming : incoming_items)
 
-def next_agent_state_from_label (a_ip : ip) (a : agent)
-  (a_next : act a.state_type)
-  (incoming : incoming_items)
+def next_agent_state_from_label (a_next : act a.state_type)
   : agent_label → option (act a.state_type × (global_state_t → global_state_t))
 | agent_label.update_own_state := match a_next with
   | (act.return new_state) := 
@@ -218,12 +225,185 @@ def next_agent_state_from_label (a_ip : ip) (a : agent)
   | _ := none
   end
 
+inductive poll_receive_dlabel (ports : list port) (sockets : list socket) (bound : ℕ) 
+   (cont : poll_result ports sockets bound → act a.state_type) : Type
+| new_connection : ∀ (sock : list.member_st (λ s : socket_info, s.server = a_ip ∧ s.new) incoming.sockets)
+    (p : ports.member),
+    sock.to_member.value.port = p.value →
+    poll_receive_dlabel
+| receive_message : ∀ (mess : incoming.messages.member)
+    (sock : sockets.member),
+    mess.value.fst = sock.value → 
+    poll_receive_dlabel
+
+inductive poll_dlabel (ports : list port) (sockets : list socket) (bound : ℕ) 
+   (cont : poll_result ports sockets bound → act a.state_type) : Type
+| timeout : poll_dlabel
+| receive : ∀ (elapsed_fin : fin bound) (rn : remote_name),
+    poll_receive_dlabel ports sockets bound cont
+    → poll_dlabel
+
+inductive dlabel : act a.state_type → Type
+| update_own_state : ∀ new_state : a.state_type, dlabel (act.return new_state)
+| connect : ∀ (rn : remote_name) cont, dlabel (act.connect rn cont)
+| send_message : ∀ sock mess cont (rn : remote_name), rn = sock
+    → dlabel (act.send_message sock mess cont)
+| poll : ∀ (ports : list port) (sockets : list socket) (bound : time) cont,
+    poll_dlabel ports sockets bound cont
+    → dlabel (act.poll ports sockets bound cont)
+    
+
+def next_agent_state_from_dlabel 
+ (a_next : act a.state_type) (la : dlabel a_next)
+  : act a.state_type × (global_state_t → global_state_t)
+:= begin
+cases la,
+{ -- update_own_state
+exact (a.loop new_state, id)
+},
+{ -- connect
+exact (
+  let s_info := socket_info.mk a_ip rn.fst rn.snd true in
+      (cont rn, add_socket s_info rn.fst))
+},
+{ -- send message
+exact (cont, add_message (a_ip, rn.snd) mess rn.fst)
+},
+{ -- poll
+induction a_1,
+  { -- timeout 
+    exact (cont (poll_result.timeout), id)
+  },
+  { -- receive
+    induction a_1,
+    { -- new connection
+      let s := sock.to_member,
+      exact (cont (poll_result.new_connection elapsed_fin p s.value.socket)
+      , lookup_updatef a_ip (λ inc, {inc with sockets := list.update_member ({s.value with new := false}) _ s}))
+    },
+    { -- receive message
+      exact (cont (poll_result.message elapsed_fin sock mess.value.snd)
+        , lookup_updatef a_ip (λ inc, {inc with messages := list.remove_member _ mess}))
+    }
+  }
+}
+end
+
+/-- Any step that we can take with a regular label, we can take 
+    with a dependent label. Therefore, it is sound to reason based
+    on the dependent-label traces.
+-/
+lemma label_dlabel_equiv (a_next : act a.state_type)
+  : ∀ ans l, next_agent_state_from_label a_next l = some ans
+  → ∃ l' : dlabel a_next, next_agent_state_from_dlabel a_next l' = ans
+:= begin
+intros ans l H,
+induction l; simp [next_agent_state_from_label] at H,
+{ cases a_next;
+    dsimp [next_agent_state_from_label] at H;
+    try { contradiction },
+  injection H with H', clear H, rw ← H',
+  fapply exists.intro, constructor, reflexivity,
+},
+{ cases a_next;
+    dsimp [next_agent_state_from_label] at H;
+    try { contradiction },
+  apply (if Hs : a_1 = a_2 then _ else _),
+  { rw (if_pos Hs) at H, subst Hs,
+    injection H with H',
+    clear H, rw ← H',
+    fapply exists.intro, constructor,
+    reflexivity,
+  },
+  { rw (if_neg Hs) at H, contradiction
+  },
+},
+{ cases a_next; 
+    dsimp [next_agent_state_from_label] at H;
+    try { contradiction },
+  apply (if Heq : (a_1 = a_3 ∧ a_2 = a_4) then _ else _),
+  { rw (if_pos Heq) at H,
+    injection H with H',
+    clear H, rw ← H',
+    fapply exists.intro, constructor,
+    reflexivity, induction Heq with H1 H2,
+    subst H1, subst H2,
+    reflexivity,
+  },
+  { rw (if_neg Heq) at H, contradiction
+  }, },
+{ cases a_next; 
+    dsimp [next_agent_state_from_label] at H;
+    try { contradiction },
+  cases a_1;
+    dsimp [next_agent_poll_state_from_label] at H,
+  { fapply exists.intro, constructor,
+    apply poll_dlabel.timeout,
+    dsimp, injection H with H',
+  },
+  { apply (if He : a_1 < bound then _ else _),
+    { rw (dif_pos He) at H,
+      induction a_4; dsimp [next_agent_receive_from_label] at H;
+         try {contradiction},
+      { -- new connection 
+        cases (list.member_st_decide (λ (s : socket_info), s.server = a_ip ∧ ↑(s.new)) 
+            (incoming.sockets));
+           dsimp [next_agent_receive_from_label] at H;
+           try { contradiction },
+        destruct (list.check_member ((a_4.to_member).value.port) ports), intros X,
+           rw X at H,
+           dsimp [next_agent_receive_from_label] at H,
+           contradiction,
+        intros p Hp, rw Hp at H,
+           dsimp [next_agent_receive_from_label] at H,
+        injection H with H'', clear H,
+        subst ans,
+        apply_in Hp list.check_member_ok,
+        fapply exists.intro, constructor,
+        apply poll_dlabel.receive, exact ⟨ _, He ⟩,
+        assumption, fapply poll_receive_dlabel.new_connection,
+        assumption, assumption, dsimp,
+        symmetry, assumption,
+        dsimp [next_agent_state_from_dlabel],
+        reflexivity,
+      },
+      { -- receive message
+        cases (list.member_st_decide (λ (p : socket × message_t), p.snd = a_4) 
+            (incoming.messages));
+          dsimp [next_agent_receive_from_label] at H;
+          try { contradiction },
+        destruct (list.check_member ((list.member.value (list.member_st.to_member a_5)).fst) sockets),
+          intros X, rw X at H,
+          dsimp [next_agent_receive_from_label] at H,
+          contradiction,
+        intros p Hp, rw Hp at H,
+           dsimp [next_agent_receive_from_label] at H,
+        injection H with H', clear H, subst ans,
+        apply_in Hp list.check_member_ok,
+        fapply exists.intro, constructor,
+        apply poll_dlabel.receive, exact ⟨ _, He ⟩,
+        assumption, fapply poll_receive_dlabel.receive_message,
+        exact a_5.to_member, assumption,
+        symmetry, assumption,
+        dsimp [next_agent_state_from_dlabel],
+        f_equal, f_equal, f_equal,
+        apply list.member_st_P_value a_5,
+      }
+    },
+    { rw (dif_neg He) at H, contradiction
+    }, 
+  }
+}
+end
+
+end
+
 def next_state_from_label (system : system_state) 
   : next_state_label → option system_state
 | (next_state_label.agent_update a_ip aupdate) := do
   a ← agents.check_member a_ip,
-  option_bind (next_agent_state_from_label a_ip a.value (system.local_state a)
-      (system.global_state a_ip) aupdate)
+  option_bind (next_agent_state_from_label a_ip a.value
+      (system.global_state a_ip) (system.local_state a) aupdate)
    $ λ p, let (next', update) := p in 
     some 
         { local_state  := lookup_update a next' system.local_state
